\subsection{Proof of Theorem \ref{theorem:smcp}}
\label{app:localization-smcp}

\begin{proof}
Consider the SMCP model described in (\ref{eq:smcp-start})-(\ref{eq:smcp-end}) with $B_l = B_r =0$ (the case with $B_l,B_r>0$ is a straightforward extension). Because the sequence of precision parameters $\pmb{\lambda}$ is known for this model, we can simply normalize $\mathbf{y}$ to have unit variance, so it is without loss of generality to assume that $\lambda_t = 1 \sforall t \in \{1,\ldots,T\}$.

Now, suppose that Assumption \ref{assumption:1} (i), (ii), (iv), and (v) (a) hold so that $t_0$ is the true location of the change-point and $b_0$ is the true shift in the $\pmb{\mu}$ at time $t_0$. If we take the ratio of the posterior probabilities of the change-point location, we get:
\begin{align*}
    \log \frac{\mathbb{P}(\gamma = t_0  \:|\: \mathbf{y} ; \tau_0,\pmb{\pi})}{\mathbb{P}(\gamma = t  \:|\: \mathbf{y} \:; \tau_0,\pmb{\pi})} &=  \log \frac{p(\mathbf{y} \:|\:\gamma = t_0 \:; \tau_0)\mathbb{P}(\gamma = t_0 \:; \pmb{\pi})/ p(\mathbf{y}\:;\tau_0,\pmb{\pi})}{p(\mathbf{y} \:|\:\gamma = t \:; \tau_0)\mathbb{P}(\gamma = t \:;\pmb{\pi})/ p(\mathbf{y}\:;\tau_0,\pmb{\pi})} \tag{Bayes' rule} \\
    &= \log \frac{p(\mathbf{y} \:|\:\gamma = t_0 \:; \tau_0)}{p(\mathbf{y} \:|\:\gamma = t \:; \tau_0)} + \log \frac{\pi_{t_0}}{\pi_t}.
\end{align*}
For some positive constants $\varepsilon$, $\delta$, and $\kappa$, suppose we can show that with high probability:
\begin{align}
    \log \frac{p(\mathbf{y} \:|\:\gamma = t_0 \:; \tau_0)}{p(\mathbf{y} \:|\:\gamma = t \:; \tau_0)} \gtrsim \log^{1+\delta} T \label{eq:thm2-result}
\end{align}
for each $t$ that satisfies $|t-t_0| > \kappa \log^{1+\varepsilon}T$. Then because $\log \frac{\pi_{t_0}}{\pi_t} = \mathcal{O}(\log T)$ by Assumption \ref{assumption:1} (v) (a), we will have:
\begin{align*}
    \log \frac{\mathbb{P}(\gamma = t_0  \:|\: \mathbf{y} ; \tau_0,\pmb{\pi})}{\mathbb{P}(\gamma = t  \:|\: \mathbf{y} \:; \tau_0,\pmb{\pi})} \gtrsim \log^{1+\delta} T 
\end{align*}
and thus:
\begin{align*}
    \max_{t \;:\; |t - t_0| > \kappa \log^{1+\varepsilon} T} \; \mathbb{P}(\gamma = t  \;|\; \mathbf{y} ; \tau_0,\pmb{\pi}) < \mathbb{P}(\gamma = t_0  \;|\; \mathbf{y} ; \tau_0,\pmb{\pi}).
\end{align*}
with probability approaching one as $T \to \infty$. 

To prove (\ref{eq:thm2-result}), we begin by directly calculating the log-marginal density of $\mathbf{y}$ as: 
\begin{align*}
    \log p(\mathbf{y} \:|\:\gamma = t ; \tau_0) &= \log \int \mathbb{P}(\mathbf{y} \:|\:b,\gamma = t) \:\; d\mathbb{P}(b;\tau_0) \\
    &= \log \int_{-\infty}^\infty (2\pi)^{-(T+1)/2} \exp\left[-\frac{\sum_{t'=1}^{t-1} y_{t'}^2 + \sum_{t'=t}^{T} (y_{t'} - b)^2}{2}\right] \tau_0^{1/2}\exp\left[-\frac{\tau_0 b^2}{2}\right] \; db \tag{(\ref{eq:dgp}) and (\ref{eq:smcp-start})-(\ref{eq:smcp-end})} \\
    &= -\frac{1}{2}\log(\tau_0 + T - t + 1) + \frac{1}{2(\tau_0 + T-t+1)}\left(\sum_{t'=t}^{T} y_{t'}\right)^2 + \log C
\end{align*}
where $C>0$ is a constant that does not depend on the value of $\gamma$. Assume that $\tau_0$ is small so that:\footnote{Formally, for any $\tau_0 >0$, we can show that for each $t$ we consider, $\Delta_t \sim p(\mathbf{y} \:|\:\gamma = t \:; \tau_0)$ as $T \to \infty$ with high probability. So if we can show there is some $\delta > 0$ such that $\log \frac{\Delta_{t_0}}{\Delta_t} > \delta-2\log(1-\delta)$, then we can show: $$\log \frac{p(\mathbf{y} \:|\:\gamma = t_0 ; \tau_0)}{p(\mathbf{y} \:|\:\gamma = t ; \tau_0)} = \log\frac{p(\mathbf{y} \:|\:\gamma = t_0 ; \tau_0)}{\Delta_{t_0}} + \log \frac{\Delta_{t_0}}{\Delta_t} + \log \frac{p(\mathbf{y} \:|\:\gamma = t ; \tau_0)}{\Delta_t} > \log(1-\delta) + \delta-2\log(1-\delta) +\log(1-\delta) > 0$$ with high probability, which is the desired result.} 
\begin{align*}
    \log p(\mathbf{y} \:|\: \gamma = t; \tau_0) &\approx -\frac{1}{2}\log(T - t + 1) + \frac{1}{2(T-t+1)}\left(\sum_{t'=t}^{T} y_{t'}\right)^2 + \log C \\
    &:= \log \Delta_t.
\end{align*}
We therefore have:
\begin{align*}
    \log \frac{\Delta_{t_0}}{\Delta_t} &= \frac{1}{2} \log \left(\frac{T-t+1}{T-t_0+1}\right) + \frac{1}{2} \left[\frac{1}{T-t_0+1}\left(\sum_{t'=t_0}^{T} y_{t'}\right)^2- \frac{1}{T-t+1}\left(\sum_{t'=t}^{T} y_{t'}\right)^2\right].
\end{align*}
To show that $\log \frac{\Delta_{t_0}}{\Delta_t} \gtrsim \log^{1+\delta} T$, with high probability, first, define the normalized terms:
\begin{align*}
    z_{t} :=
    \begin{cases}
        y_t, & \text{if } t < t_0, \\
        y_t - b_0, & \text{if } t \geq t_0.
    \end{cases}
\end{align*}
Then there are two cases to consider:

\subsubsection*{Case 1: $t > t_0$.}

First, since $T-t +1\geq 1$ and $T-t_0+1 < T$, by the monotonicity of log we have: 
\begin{align*}
    \log \left(\frac{T-t+1}{T-t_0+1}\right) \geq -\log(T-t_0+1) > -\log T.
\end{align*}
Therefore, we have:
\begin{align*}
    \log \frac{\Delta_{t_0}}{\Delta_t} &> -\frac{1}{2} \log T + \frac{1}{2} \left[\frac{1}{T-t_0+1}\left(\sum_{t'=t_0}^{T} y_{t'}\right)^2- \frac{1}{T-t+1}\left(\sum_{t'=t}^{T} y_{t'}\right)^2\right]. 
\end{align*}
If we define the following terms:
\begin{align*}
    \overline{z}_{t_0:T} &:= \frac{1}{T-t_0+1}\sum_{t'=t_0}^T z_{t'} \\
    \overline{z}_{t:T} &:= \frac{1}{T-t+1}\sum_{t'=t}^T z_{t'}
\end{align*}
then we can write:
\small
\begin{align*}
    \frac{1}{T-t_0+1}\left(\sum_{t'=t_0}^{T} y_{t'}\right)^2- \frac{1}{T-t+1}\left(\sum_{t'=t}^{T} y_{t'}\right)^2 &= (t-t_0)b_0^2 + 2b_0\sum_{t'=t_0}^{t-1}z_{t'} + (T-t_0+1) \overline{z}^2_{t_0:T} - (T-t+1)\overline{z}^2_{t:T}.
\end{align*}
\normalsize
Since $(T-t_0+1) \overline{z}^2_{t_0:T} > 0$, we now have: 
\begin{align}
    \log \frac{\Delta_{t_0}}{\Delta_t} &> -\frac{1}{2} \log T + \frac{1}{2} \left[(t-t_0)b_0^2 + 2b_0\sum_{t'=t_0}^{t-1}z_{t'} - (T-t+1)\overline{z}^2_{t:T}\right].\label{eq:thm1-cs1-bd}
\end{align}
Let $\varepsilon > 0$ be given, and define the event: 
\begin{align*}
    \mathcal{E}_1 &:= \left\{\left|\sum_{t'=t_0}^{t-1} z_{t'}\right| < \frac{(t-t_0) |b_0|}{4}, \; \sforall t \text{ s.t. } t > t_0 + 64 \log^{1+\varepsilon}T\right\}.
\end{align*}
By Assumption \ref{assumption:1} there exists some $\varphi \in (0,\varepsilon/2)$ such that $|b_0| \geq \log^{-\varphi/2}T$. We also have that:
\begin{align*}
    \sum_{t'=t_0}^{t-1} z_{t'} \sim \mathcal{N}(0,t-t_0)
\end{align*}
and thus: 
\begin{align}
    \mathbb{P}\left(\left|\sum_{t'=t_0}^{t-1} z_{t'}\right| \geq \frac{(t-t_0) |b_0|}{4}\right) &\leq \mathbb{P}\left(\left|\sum_{t'=t_0}^{t-1} z_{t'}\right| \geq \frac{(t-t_0) \log^{-\varphi/2}T}{4}\right) \tag{$|b_0| \geq \log^{-\varphi/2}T$} \\
    &\leq 2 \exp\left[- \frac{(t-t_0)\log^{-\varphi}T}{32}\right] \tag{Chernoff Bound}\\
    &\leq 2 \exp\left[- 2 \log^{1+\varepsilon-\varphi}T\right] \tag{$t_0 - t > 64 \log^{1 + \varepsilon} T$} \\
    &\leq 2 \exp\left[- 2 \log T\right] \tag{$\varepsilon - \varphi > 0 \implies \log^{1+\varepsilon-\varphi}T > \log T$ for $T > e$} \\
    &= \frac{2}{T^2} \label{bd:E1-inter}
\end{align}
Using the bound in (\ref{bd:E1-inter}) we get:
\begin{align}
    \mathbb{P}(\mathcal{E}^c_1) &= \mathbb{P}\left(\bigcup_{ t \;:\; t > t_0 + 64 \log^{1+\varepsilon}T} \left\{\left|\sum_{t'=t_0}^{t-1} z_{t'}\right| \geq \frac{(t-t_0)|b_0|}{4}\right\} \right) \notag \\
    &\leq \sum_{ t \;:\; t > t_0 + 64 \log^{1+\varepsilon}T} \mathbb{P}\left(\left|\sum_{t'=t_0}^{t-1} z_{t'}\right| \geq \frac{(t-t_0) |b_0|}{4}\right) \tag{union bound} \\
    &\leq \sum_{ t \;:\; t > t_0 + 64 \log^{1+\varepsilon}T} \frac{2}{T^2} \tag{by (\ref{bd:E1-inter})}\\
    &\leq \frac{2(1-c)}{T} \label{bd:E1}
\end{align}
where (\ref{bd:E1}) follows from bounding the number of terms in the previous summation with $(1-c)T$. This holds since $t > t_0 + 64 \log^{1+\varepsilon}T > t_0 + 1$ for large $T$ and $T - t_0 \leq (1-c)T$ by Assumption \ref{assumption:1} (i). 

Now define the event:
\begin{align*}
    \mathcal{E}_2 &:= \left\{\left|(T-t+1)\overline{z}^2_{t:T} - 1\right| < 16 \log T, \; \sforall t \in\{t_0+1,\ldots,T\}\right\}.
\end{align*}
Since $\overline{z}_{t:T}\sim \mathcal{N}(0,(T-t+1)^{-1}) \sforall t > t_0$, we have $(T-t+1)\overline{z}^2_{t:T}\sim \chi_1^2$ for each $t > t_0$, so by the $\chi^2$-concentration inequality (\ref{eq:chi2-ineq}) we get: 
\begin{align}
    \mathbb{P}\left(\left|(T-t+1)\overline{z}^2_{t:T} - 1\right| \geq 16 \log T\right) &\leq 2\exp\left[-2\log T\right] \notag \\
    &= \frac{2}{T^2}. \label{bd:E2-inter}
\end{align}
Using this bound we get:
\begin{align}
    \mathbb{P}(\mathcal{E}^c_2) &= \mathbb{P}\left(\bigcup_{t = t_0 +1}^T \left\{\left|(T-t+1)\overline{z}^2_{t_0:T} - 1\right| \geq 8 \log^{1+\varepsilon}T\right\} \right) \notag \\
    &\leq \sum_{t = t_0 +1}^T \mathbb{P}\left(\left|(T-t+1)\overline{z}^2_{t_0:T} - 1\right| \geq 8 \log^{1+\varepsilon-\varphi}T\right) \tag{union bound} \\
    &\leq \sum_{t = t_0 +1}^T \frac{2}{T^2} \tag{by (\ref{bd:E2-inter})} \\
    &\leq \frac{2(1- c)}{T} \label{bd:E2} 
\end{align}
where the last bound in (\ref{bd:E2}) again follows the fact that there are at most $(1-c)T$ terms in the sum. If we define the joint event $\mathcal{E} := \mathcal{E}_1 \cap \mathcal{E}_2$, then we have:
\begin{align*}
    \mathbb{P}(\mathcal{E}) &= 1 - \mathbb{P}(\mathcal{E}^c_1 \cup \mathcal{E}^c_2) \\
    &\geq 1 - \mathbb{P}(\mathcal{E}^c_1) - \mathbb{P}(\mathcal{E}^c_2) \tag{Union Bound}  \\
    &\geq 1 - \frac{4(1-c)}{T} \tag{by (\ref{bd:E1}) and (\ref{bd:E2})}.
\end{align*}
So $\lim_{T\to\infty}\mathbb{P}(\mathcal{E}) = 1$. Now assume that we are on $\mathcal{E}$ and $t > t_0 + 64 \log^{1+\varepsilon}T$, then going back to the bound in (\ref{eq:thm1-cs1-bd}) we have:
\begin{align*}
    \log \frac{\Delta_{t_0}}{\Delta_t} &> -\frac{1}{2} \log T + \frac{1}{2} \left[(t-t_0)b_0^2 + 2b_0\sum_{t'=t_0}^{t-1}z_{t'} - (T-t+1)\overline{z}^2_{t:T}\right] \\
    &> -\frac{1}{2} \log T + \frac{1}{2} \left[\frac{(t-t_0)}{2}b_0^2 - (T-t+1)\overline{z}^2_{t:T}\right] \tag{$2b_0\sum_{t'=t_0}^{t-1}z_{t'} \geq - |2b_0\sum_{t'=t_0}^{t-1}z_{t'}| > - (t-t_0)b_0^2/ 2$ on $\mathcal{E}_1$} \\
    &\geq -\frac{1}{2} \log T + \frac{1}{2} \left[\frac{(t-t_0)}{2}\log^{-\varphi}T - (T-t+1)\overline{z}^2_{t:T}\right] \tag{$b_0^2 \geq \log^{-\varphi}T$} \\
    &> -\frac{1}{2} \log T + \frac{1}{2} \left[32\log^{1+\varepsilon- \varphi}T - (T-t+1)\overline{z}^2_{t:T} + 1 - 1\right] \tag{$t-t_0 > 64 \log^{1+\varepsilon}T$} \\
    &> 16\log^{1+\varepsilon-\varphi}T - \left(8 + \frac{1}{2}\right) \log T - \frac{1}{2}
\end{align*}
where in the last line used the fact that on $\mathcal{E}$:
\begin{align*}
    1-(T-t+1)\overline{z}^2_{t:T} \geq - | (T-t+1)\overline{z}^2_{t:T} - 1| > -16\log T.
\end{align*}
Then we have $\log \frac{\Delta_{t_0}}{\Delta_t} \gtrsim \log^{1+\delta} T$ on $\mathcal{E}$.

\subsubsection*{Case 2: $t < t_0$.}

We can write:
\small
\begin{align*}
    \frac{1}{T-t_0+1}\left(\sum_{t'=t_0}^{T} y_{t'}\right)^2 - \frac{1}{T-t+1}\left(\sum_{t'=t}^{T} y_{t'}\right)^2 &= \frac{1}{T-t_0+1}\left(\sum_{t'=t_0}^{T} z_{t'} + (T-t_0+1)b_0\right)^2 \\
    &\quad - \frac{1}{T-t+1}\left(\sum_{t'=t}^{t_0-1} z_{t'} + \sum_{t'=t_0}^{T} z_{t'} + (T-t_0+1)b_0\right)^2 \\ 
    &= \frac{(T-t_0+1)(t_0 - t) b_0^2}{T-t+1} \\
    &\quad + \frac{1}{T-t_0+1}\left(\sum_{t'=t_0}^{T} z_{t'}\right)^2 -\frac{1}{T-t+1}\left(\sum_{t'=t}^{T} z_{t'}\right)^2\\
    &\quad  + 2(t_0 - t) b_0\left(\frac{1}{T-t+1}\sum_{t'=t}^{T} z_{t'} - \frac{1}{t_0-t}\sum_{t'=t}^{t_0-1} z_{t'}\right)
\end{align*}
\normalsize
Since $T-t+1 < T$ and $T - t_0 + 1 > cT$ by Assumption \ref{assumption:1} (i), we have:
\begin{align*}
    \frac{(T - t_0 + 1)(t_0-t)b_0^2}{T-t+1} &> c (t_0-t) b_0^2 
\end{align*}
and thus:
\begin{align*}
    \frac{1}{T-t_0+1}\left(\sum_{t'=t_0}^{T} y_{t'}\right)^2 - \frac{1}{T-t+1}\left(\sum_{t'=t}^{T} y_{t'}\right)^2 &> c(t_0 - t)b_0^2 -\frac{1}{T-t+1}\left(\sum_{t'=t}^{T} z_{t'}\right)^2\\
    &\quad  - 2(t_0 - t) |b_0|\left(\frac{1}{T-t+1}\left|\sum_{t'=t}^{T} z_{t'}\right| + \frac{1}{t_0-t}\left|\sum_{t'=t}^{t_0-1} z_{t'}\right|\right)
\end{align*}
Noting that $t < t_0$ implies $T - t + 1 > T - t_0 + 1$ and thus $ \log \frac{T-t+1}{T-t_0+1} > 0$, we have:
\small
\begin{align}
    \log \frac{\Delta_{t_0}}{\Delta_t} &= \frac{1}{2} \log \left(\frac{T-t+1}{T-t_0+1}\right) + \frac{1}{2} \left[\frac{1}{T-t_0+1}\left(\sum_{t'=t_0}^{T} y_{t'}\right)^2- \frac{1}{T-t+1}\left(\sum_{t'=t}^{T} y_{t'}\right)^2\right] \notag \\
    &> \frac{c (t_0-t)b_0^2 }{2} - c(t_0 -t) |b_0| \left(\frac{1}{T-t+1}\left|\sum_{t'=t}^{T} z_{t'}\right| + \frac{1}{t_0-t}\left|\sum_{t'=t}^{t_0-1} z_{t'}\right|\right) -\frac{1}{2(T-t+1)}\left(\sum_{t'=t}^{T} z_{t'}\right)^2 \label{eq:thm1-cs2-bd}
\end{align}
\normalsize
Again, let $\varepsilon > 0$ be given, and define the events: 
\begin{align*}
    \Omega_1 &:= \left\{\frac{1}{t_0-t}\left|\sum_{t'=t}^{t_0-1} z_{t'}\right| < \frac{|b_0|}{8}, \; \sforall t \text{ s.t. } t < t_0 - 256 \log^{1+\varepsilon}T\right\} \\
    \Omega_2 &:= \left\{\frac{1}{T-t+1}\left|\sum_{t'=t}^T z_{t'}\right| < \frac{|b_0|}{8}, \; \sforall t \text{ s.t. } t < t_0 \right\}.
\end{align*}
By Assumption \ref{assumption:1} there exists some $\varphi \in (0,\varepsilon/2)$ such that $|b_0| \geq \log^{-\varphi/2}T$. We also have:
\begin{align*}
    \sum_{t'=t}^{t_0-1} z_{t'} &\sim \mathcal{N}(0, t_0 - t) 
\end{align*}
which gives:
\begin{align}
    \mathbb{P}\left(\frac{1}{t_0-t}\left|\sum_{t'=t}^{t_0-1} z_{t'}\right| > \frac{|b_0|}{4}\right) &\leq \mathbb{P}\left(\frac{1}{t_0-t}\left|\sum_{t'=t}^{t_0-1} z_{t'}\right| > \frac{\log^{-\varphi/2}T}{4}\right) \tag{$|b_0| \geq \log^{-\varphi/2}T$} \\
    &\leq 2 \exp\left[- \frac{(t_0-t)\log^{-\varphi}T}{128}\right] \tag{Chernoff Bound}\\
    &\leq 2 \exp\left[- 2\log^{1+\varepsilon-\varphi}T\right] \tag{$t_0 - t > 256\log^{1+\varepsilon} T$} \\
    &\leq 2 \exp\left[- 2\log^{1+\varepsilon-\varphi}T\right] \tag{$\varepsilon-\varphi > 0 \implies \log^{1+\varepsilon-\varphi}T > \log T$ for $T > e$}\\ 
    &= \frac{2}{T^2} \label{bd:O1-inter} 
\end{align}
Similarly, we have:
\begin{align*}
    \sum_{t'=t}^{T} z_{t'} &\sim \mathcal{N}(0, T - t + 1)
\end{align*}
so:
\begin{align}
    \mathbb{P}\left(\frac{1}{T-t+1}\left|\sum_{t'=t}^T z_{t'}\right| > \frac{ |b_0|}{8}\right) &\leq \mathbb{P}\left(\frac{1}{T-t+1}\left|\sum_{t'=t}^T z_{t'}\right| > \frac{\log^{-\varphi/2}T}{4}\right) \tag{$|b_0| \geq \log^{-\varphi/2}T$} \\
    &\leq 2 \exp\left[- \frac{(T-t + 1)\log^{-\varphi}T}{128}\right] \tag{Chernoff Bound}\\
    &\leq 2 \exp\left[- \frac{cT\log^{-\varphi}T}{128}\right] \label{bd:O2-inter} 
\end{align}
where the last line in (\ref{bd:O2-inter}) follows from the fact that $T-t+1> T-t_0 > cT$. Using these bounds, we have:
\begin{align}
    \mathbb{P}(\Omega^c_1) &= \mathbb{P}\left(\bigcup_{ t \;:\; t < t_0 - 256 \log^{1+\varepsilon}T} \left\{
    \frac{1}{t_0-t}\left|\sum_{t'=t}^{t_0-1} z_{t'}\right| \geq \frac{|b_0|}{8}\right\} \right) \notag \\
    &\leq \sum_{ t \;:\; t < t_0 - 256 \log^{1+\varepsilon}T} \mathbb{P}\left(\frac{1}{t_0-t}\left|\sum_{t'=t}^{t_0-1} z_{t'}\right| \geq \frac{|b_0|}{8}\right) \tag{union bound} \\
    &\leq \sum_{ t \;:\; t < t_0 - 256 \log^{1+\varepsilon}T} \frac{2}{T^2} \tag{by (\ref{bd:O1-inter})}\\
    &\leq \frac{2(1-c)}{T} \label{bd:O1}
\end{align}
where the last bound in (\ref{bd:O1}) follows from the fact that $t < t_0 < (1-c)T$, which bounds the number of terms in the sum. Similarly:
\begin{align}
    \mathbb{P}(\Omega^c_2) &= \mathbb{P}\left(\bigcup_{ t \;:\; t < t_0} \left\{
    \frac{1}{T-t+1}\left|\sum_{t'=t}^T z_{t'}\right| \geq \frac{|b_0|}{8}\right\} \right) \notag \\
    &\leq \sum_{ t \;:\; t < t_0} \mathbb{P}\left(\frac{1}{T-t+1}\left|\sum_{t'=t}^T z_{t'}\right| \geq \frac{|b_0|}{8}\right) \tag{union bound} \\
    &\leq \sum_{ t \;:\; t < t_0 } 2 \exp\left[- \frac{cT\log^{-\varphi}T}{128}\right] \tag{by (\ref{bd:O2-inter})}\\
    &\leq 2 (1-c)\exp\left[\log T - \frac{cT\log^{-\varphi}T}{128}\right]. \label{bd:O2}
\end{align}
Lastly, if we define the event:
\begin{align*}
    \Omega_3 &:= \left\{\left|\frac{1}{(T-t+1)}\left(\sum_{t'=t}^{T} z_{t'}\right)^2 - 1\right| < 16 \log T, \; \sforall t \in\{1,\ldots,t_0-1\}\right\}
\end{align*}
then since: 
\begin{align*}
    \frac{1}{(T-t+1)}\left(\sum_{t'=t}^{T} z_{t'}\right)^2 \sim \chi_1^2,\; \sforall t < t_0
\end{align*}
by the $\chi^2$-concentration inequality (\ref{eq:chi2-ineq}) we get: 
\begin{align}
    \mathbb{P}\left(\left|\frac{1}{(T-t+1)}\left(\sum_{t'=t}^{T} z_{t'}\right)^2 - 1\right| \geq 16 \log T\right) &\leq 2\exp\left[-2\log T\right] \notag \\
    &= \frac{2}{T^2}. \label{bd:O3-inter}
\end{align}
Using this bound we get:
\begin{align}
    \mathbb{P}(\Omega^c_3) &= \mathbb{P}\left(\bigcup_{t=1}^{t_0-1} \left\{\left|\frac{1}{(T-t+1)}\left(\sum_{t'=t}^{T} z_{t'}\right)^2 - 1\right| \geq 16 \log T\right\} \right) \notag \\
    &\leq \sum_{t = 1}^{t_0-1} \mathbb{P}\left(\left|\frac{1}{(T-t+1)}\left(\sum_{t'=t}^{T} z_{t'}\right)^2 - 1\right| > 16 \log T\right) \tag{union bound} \\
    &\leq \sum_{t = 1}^{t_0-1} \frac{2}{T^2} \tag{by (\ref{bd:O3-inter})} \\
    &\leq \frac{2(1- c)}{T} \label{bd:O3} 
\end{align}
If we define the joint event $\Omega := \bigcap_{i=1}^3 \Omega_i$, then we have:
\begin{align*}
    \mathbb{P}(\Omega) &= 1 - \mathbb{P}(\Omega^c_1 \cup \Omega^c_2 \cup \Omega^c_3) \\
    &\geq 1 - \mathbb{P}(\Omega^c_1) - \mathbb{P}(\Omega^c_2) - \mathbb{P}(\Omega^c_3) \tag{Union Bound}  \\
    &\geq 1 - 2 (1-c)\exp\left[\log T - \frac{cT\log^{-\varphi}T}{128}\right] - \frac{4(1-c)}{T} \tag{by (\ref{bd:O1}), (\ref{bd:O2}), and (\ref{bd:O3})}.
\end{align*}
So $\lim_{T\to\infty}\mathbb{P}(\Omega) = 1$. Now assume that we are on $\Omega$ and $t > t_0 + 256 \log^{1+\varepsilon}T$, then going back to the bound in (\ref{eq:thm1-cs2-bd}) we have:
\begin{align*}
    \log \frac{\Delta_{t_0}}{\Delta_t} &> \frac{c (t_0-t)b_0^2 }{2} - c(t_0 -t) |b_0| \left(\frac{1}{T-t+1}\left|\sum_{t'=t}^{T} z_{t'}\right| + \frac{1}{t_0-t}\left|\sum_{t'=t}^{t_0-1} z_{t'}\right|\right) -\frac{1}{2(T-t+1)}\left(\sum_{t'=t}^{T} z_{t'}\right)^2 \\
    &> \frac{c (t_0-t)b_0^2 }{2} - c(t_0 -t) |b_0| \left(\frac{1}{T-t+1}\left|\sum_{t'=t}^{T} z_{t'}\right| + \frac{1}{t_0-t}\left|\sum_{t'=t}^{t_0-1} z_{t'}\right|\right) -8\log T - \frac{1}{2} \tag{$\frac{1}{2(T-t+1)}\left(\sum_{t'=t}^{T} z_{t'}\right)^2 < 16\log T + 1$ on $\Omega$} \\
    &> \frac{c (t_0-t)b_0^2 }{2} - c(t_0 -t) |b_0| \left(\frac{|b_0|}{8} + \frac{|b_0|}{8}\right) -8\log T - \frac{1}{2} \tag{$\frac{1}{T-t+1}\left|\sum_{t'=t}^{T} z_{t'}\right| < \frac{b_0}{8}$ and $\frac{1}{t_0-t}\left|\sum_{t'=t}^{t_0-1} z_{t'}\right| < \frac{b_0}{8}$ on $\Omega$} \\
    &> \frac{c}{4}\log^{1+\varepsilon-\varphi} T -8\log T - \frac{1}{2}
\end{align*}
where the last line follows from the fact that $b_0^2 \geq \log^{-\varphi} T$ and $t_0 - t > \log^{1+\varepsilon} T$. So if we again let $\delta = \varepsilon -\varphi >0$, then we have $\log \frac{\Delta_{t_0}}{\Delta_t} \gtrsim \log^{1+\delta} T$ on $\Omega$.

Combining the case of $t > t_0$ and $t < t_0$, again by the union bound have have:
\begin{align*}
    \mathbb{P}(\mathcal{E} \cap \Omega) = 1 - \mathbb{P}(\mathcal{E}^c) -\mathbb{P}(\Omega^c) \to 1
\end{align*}
and if we let $\kappa = 256$, then on $\mathcal{E} \cap \Omega$ we have:
\begin{align*}
    \max_{t \;:\; |t - t_0| > \kappa \log^{1+\varepsilon} T} \; \mathbb{P}(\gamma = t  \;|\; \mathbf{y} ; \tau_0,\pmb{\pi}) < \mathbb{P}(\gamma = t_0  \;|\; \mathbf{y} ; \tau_0,\pmb{\pi}).
\end{align*}
\end{proof}