\subsection{Theorem \ref{theorem:alpha-mixing} Event Bounds}

\begin{lemma}[Theorem \ref{theorem:alpha-mixing} Event Bounds]\label{lemma:thm4-event-bound}

Let $\{y_t\}_{t\geq 1}$ be a univariate sequence of random variables satisfying Assumption \ref{assumption:alpha-mixing}. Let $\E[y_t] = b_0\mathbbm{1}\{t\geq t_0\}$ and $\normalfont{\Var}(y_t) = (s_0^2)^{\mathbbm{1}\{t\geq t_0\}}$, with $b_0 \in \mathbb{R}$ and $s_0 > 0$ so that it is possible that $b_0 = 0$ or $s_0 = 1$. Define the standardized term $z_t:= \frac{y_t - b_0\mathbbm{1}\{t\geq t_0\}}{s_0^{\mathbbm{1}\{t\geq t_0\}}}$ and the functions $f_1$ and $f_2$ as in (\ref{eq:f1-signal-fn}) and (\ref{eq:f2-signal-fn}), then for any $\delta > 0$, there exist some universal constants $\kappa, C > 0$ such that for any $T\in\mathbb{N}$ and $t_0$ such that $\min\{t_0,T-t_0\} > \log^{2+\varepsilon} T$ for some $\varepsilon > 2\delta$, if we define the set:
\begin{align*}
    \mathcal{T}_{\kappa,\delta}:= \left\{1\leq t \leq T - \lfloor\log^{2 + \delta} T\rfloor \::\: |t_0 - t| > \frac{\kappa\log^{2 + \delta} T}{b^2_0 + \min\{f_1(s_0^2),f_2(s_0^2)\}} \right\}
\end{align*}
and the events: 
\begin{align*}
    \mathcal{E}_1 &:= \bigcap_{t \in \mathcal{T}_{\kappa, \delta}} \left\{\left|\sum_{t'=\min\{t_0,t\}}^{\max\{t_0,t\}-1} z_{t'}\right| < C\sqrt{|t_0-t|}\log^{1+\frac{\delta}{4}} T\right\}, \\
    \mathcal{E}_2 &:= \bigcap_{t \in \mathcal{T}_{\kappa, \delta}} \left\{\left|\sum_{t'=\min\{t_0,t\}}^{\max\{t_0,t\}-1} (z_{t'}^2 - 1) \right| <  C\sqrt{|t_0-t|}\log^{1+\frac{\delta}{4}} T  \right\},  \\
    \mathcal{E}_3 &:= \bigcap_{t=1}^{T- \lfloor\log^{2 +\delta} T\rfloor }  \left\{\left|\sum_{t'=t}^{T} z_{t'}\right| < C\sqrt{T-t+1}\log^{1+\frac{\delta}{4}} T  \right\}, \\
    \mathcal{E}_4 &:= \bigcap_{t=1}^{T- \lfloor\log^{2 +\delta} T \rfloor} \left\{\left|\sum_{t'=t}^{T} (z_{t'}^2 - 1) \right| <  C\sqrt{T-t+1}\log^{1+\frac{\delta}{4}} T  \right\},
\end{align*}
and the joint event $\mathcal{E} := \bigcap_{i=1}^4 \mathcal{E}_i$, then we will have $\lim_{T\to\infty} \Pr(\mathcal{E}) = 1$. 
\end{lemma}

\begin{proof}

First, by Assumption \ref{assumption:alpha-mixing} there are stochastic processes $\{y_{0,t}\}_{t \geq 1}$ and $\{y_{1,t}\}_{t \geq 1}$ such that $y_{0,t} \sim F_0$, and $y_{1,t} \sim F_1$, $y_t := y_{0,t} \mathbbm{1}\{t < t_0\}  + y_{1,t}\mathbbm{1}\{t \geq t_0\}$, and:
    \begin{enumerate}[label=(\roman*)]
        \item $\{y_{0,t}\}_{t \geq 1}$ and $\{y_{1,t}\}_{t \geq 1}$ are $\alpha$-mixing processes with respective coefficients $\{\alpha_{0,k}\}_{k\geq 1}$ and $\{\alpha_{1,k}\}_{k\geq 1}$ that satisfy $\max\{\alpha_{0,k}, \alpha_{1,k}\} \leq e^{-C k}$ for some $C > 0$.
        \item There exist constants $\delta_1, D_1 > 0$ such that $\sup_{t \geq 1} \max\{\E\left[|y_{0,t}|^{4+\delta_1}\right],\;\E\left[|y_{1,t}|^{4+\delta_1}\right]\}\leq D_1.$  
    \end{enumerate}
Let $z_{0,t} := y_{0,t}$ and $z_{1,t} := \frac{y_{1,t} - b_0}{s_0}$. Since $|y_{0,t}|^{2+\frac{\delta_1}{2}} \leq 1 + |y_{0,t}|^{4+\delta_1}$ we have:
\begin{align*}
    \E\left[\left|z_{0,t}\right|^{2 + \frac{\delta_1}{2}}\right] = \E\left[\left|y_{0,t}\right|^{2 + \frac{\delta_1}{2}}\right] < 1 + \E\left[\left|y_{0,t}\right|^{4 + \delta_1}\right] < 1 + D_1.
\end{align*}
Next:
\begin{align*}
    \E\left[\left|z^2_{0,t} -1 \right|^{2+\frac{\delta_1}{2}}\right] &\leq \E\left[\left(z_{0,t}^2 + 1\right)^{2+\frac{\delta_1}{2}}\right]\\
    &\leq 2^{2+\frac{\delta_1}{2}}\E\left[\frac{z_{0,t}^{4+\delta_1} + 1}{2}\right] \tag{$x^{2+\frac{\delta_1}{2}}$ is convex}\\
    &=2^{1+\frac{\delta_1}{2}}\left(\E\left[y_{0,t}^{4+\delta_1} \right]+ 1\right) \\
    &< 2^{1+\frac{\delta_1}{2}}(D_1 + 1).    
\end{align*}
If Assumption \ref{assumption:mean} holds, there is some $\overline{b} > 0$ such that $|b_0| \leq \overline{b}$ (if Assumption \ref{assumption:mean} does not hold then we can set $\overline{b}=0$) and if Assumption \ref{assumption:scale} holds, there is some $\underline{s}^2 > 0$ such that $s^2_0 \geq \underline{s}^2$ (if Assumption \ref{assumption:scale} does not hold, then we can set $\underline{s}^2=1$). Therefore:
\begin{align*}
    \E\left[\left|z^2_{1,t} -1 \right|^{2+\frac{\delta_1}{2}}\right] &\leq \E\left[\left(z_{1,t}^2 + 1\right)^{2+\frac{\delta_1}{2}}\right]\\
    &\leq 2^{1+\frac{\delta_1}{2}}\left(\E\left[z_{1,t}^{4+\delta_1} \right]+ 1\right) \tag{$x^{2+\frac{\delta_1}{2}}$ is convex} \\
    &= 2^{1+\frac{\delta_1}{2}}\left(\E\left[\left|\frac{y_{1,t} - b_0}{s_0}\right|^{4+\delta_1}\right] + 1\right) \\
    &\leq 2^{1+\frac{\delta_1}{2}}\left(\frac{\E\left[\left(|y_{1,t}| + |b_0| \right)^{4+\delta_1}\right]}{s_0^{4+\delta_1}}+ 1\right)  \\
    &\leq 2^{1+\frac{\delta_1}{2}}\left(\frac{2^{3+\delta_1}\E\left[|y_{1,t}|^{4+\delta_1} + |b_0|^{4+\delta_1}\right]}{s_0^{4+\delta_1}} + 1\right) \tag{$x^{4+\delta_1}$ is convex} \\
    &\leq 2^{1+\frac{\delta_1}{2}}\left(\frac{2^{3+\delta_1}(D_1 + \overline{b}^{4+\delta_1})}{\underline{s}^{4+\delta_1}} + 1 \right)
\end{align*}
and:
\begin{align*}
    \E\left[\left|z_{1,t}\right|^{2 + \frac{\delta_1}{2}}\right] \leq 1 + \E\left[\left|z_{1,t}\right|^{4 + \delta_1}\right] \leq 1+2^{1+\frac{\delta_1}{2}}\left(\frac{2^{3+\delta_1}(D_1 + \overline{b}^{4+\delta_1})}{\underline{s}^{4+\delta_1}} + 1 \right)
\end{align*}
Next, since $z_{1,t}$ is a continuous and therefore measurable function of $y_{1,t}$, for any $t \geq 1$ and $k \geq 0$, we have:
\begin{align*}
    \sigma(\{z_{1,t'}\}_{t'\leq t}) &\subseteq \sigma(\{y_{1,t'}\}_{t'\leq t}) \\
    \sigma(\{z_{1,t'}\}_{t'\geq t+k}) &\subseteq \sigma(\{y_{1,t'}\}_{t'\geq t+k})
\end{align*}
which implies:
\begin{align*}
    \alpha_k(\{z_{1,t}\}_{t\geq 1}) \leq \alpha_k(\{y_{1,t}\}_{t\geq 1}) \leq e^{-Ck}.
\end{align*}
Similarly, $z^2_{0,t} - 1$ is a continuous and therefore measurable function of $y_{0,t}$, and thus:
\begin{align*}
    \sigma(\{z^2_{0,t'} - 1\}_{t'\leq t}) &\subseteq \sigma(\{y_{0,t'}\}_{t'\leq t}) \\
    \sigma(\{z^2_{0,t'} - 1\}_{t'\geq t+k}) &\subseteq \sigma(\{y_{0,t'}\}_{t'\geq t+k})
\end{align*}
and thus:
\begin{align*}
    \alpha_k(\{z^2_{0,t} - 1\}_{t\geq 1}) \leq \alpha_k(\{y_{0,t}\}_{t\geq 1}) \leq e^{-Ck}.
\end{align*}
An identical argument shows that:
\begin{align*}
    \alpha_k(\{z^2_{1,t} - 1\}_{t\geq 1}) \leq \alpha_k(\{z_{1,t}\}_{t\geq 1}) \leq e^{-Ck}.
\end{align*}
Therefore, $\{z_{0,t}\}_{t\geq1}$, $\{z_{1,t}\}_{t\geq1}$, $\{z^2_{0,}-1\}_{t\geq1}$, and $\{z^2_{1,t}-1\}_{t\geq1}$ are all $\alpha$-mixing processes with moments and coefficients that satisfy the conditions of Lemma \ref{lemma:Padilla23}. For $C_1 >0$, we can write:
\small
\begin{align*}
    \Pr\left(\mathcal{E}_1^c\right) &= \Pr\left(\bigcup_{t \in \mathcal{T}_{\kappa, \delta}} \left\{\left|\sum_{t'=\min\{t_0,t\}}^{\max\{t_0,t\}-1} z_{t'}\right| \geq C_1\sqrt{|t_0-t|}\log^{1+\frac{\delta}{4}} T\right\} \right) \\
    &\leq \Pr\left(\bigcup_{t \in \mathcal{T}_{\kappa, \delta} \::\: t < t_0} \left\{\left|\sum_{t'=t}^{t_0-1} z_{t'}\right| \geq C_1\sqrt{t_0-t}\log^{1+\frac{\delta}{4}} T\right\} \right) + \Pr\left(\bigcup_{t \in \mathcal{T}_{\kappa, \delta} \::\: t > t_0} \left\{\left|\sum_{t'=t_0}^{t-1} z_{t'}\right| \geq C_1\sqrt{t-t_0}\log^{1+\frac{\delta}{4}} T\right\} \right) \tag{union bound} \\
    &\leq \Pr\left(\bigcup_{t = 1}^{t_0-1} \left\{\left|\sum_{t'=t}^{t_0-1} z_{t'}\right| \geq C_1\sqrt{t_0-t}\log^{1+\frac{\delta}{4}} T\right\} \right) + \Pr\left(\bigcup_{t = t_0+1}^T \left\{\left|\sum_{t'=t_0}^{t-1} z_{t'}\right| \geq C_1\sqrt{t-t_0}\log^{1+\frac{\delta}{4}} T\right\} \right) \\
    &= \Pr\left(\bigcup_{t = 1}^{t_0-1} \left\{\left|\sum_{t'=t}^{t_0-1} z_{0,t'}\right| \geq C_1\sqrt{t_0-t}\log^{1+\frac{\delta}{4}} T\right\} \right) + \Pr\left(\bigcup_{t = t_0+1}^T \left\{\left|\sum_{t'=t_0}^{t-1} z_{1,t'}\right| \geq C_1\sqrt{t-t_0}\log^{1+\frac{\delta}{4}} T\right\} \right) \tag{$z_{t'} = z_{0,t'} \mathbbm{1}\{t' < t_0\}  + z_{1,t'}\mathbbm{1}\{t' \geq t_0\}$}
\end{align*}
\normalsize
Since $\{z_{0,t}\}_{t\geq1}$ and $\{z_{1,t}\}_{t\geq1}$ satisfy the conditions of Lemma \ref{lemma:alpha-mix-sum}, for some $K_1,K_2 > 0$ we have:
\begin{align*}
    \Pr\left(\bigcup_{t = 1}^{t_0-1} \left\{\left|\sum_{t'=t}^{t_0-1} z_{0,t'}\right| \geq K_1\sqrt{t_0-t}\log^{1+\frac{\delta}{4}} T\right\} \right) &\leq \frac{1}{\sqrt{\log^\delta T}} \\
    \Pr\left(\bigcup_{t = t_0+1}^T \left\{\left|\sum_{t'=t_0}^{t-1} z_{1,t'}\right| \geq K_2\sqrt{t-t_0}\log^{1+\frac{\delta}{4}} T\right\} \right) &\leq \frac{1}{\sqrt{\log^\delta T}}
\end{align*}
So for $C_1 > \max\{K_1,K_2\}$ we get $\Pr\left(\mathcal{E}_1^c\right) \leq \frac{2}{\sqrt{\log^\delta T}}$. Since $\{z^2_{0,t}-1\}_{t\geq1}$ and $\{z^2_{1,t}-1\}_{t\geq1}$ also satisfy the conditions of Lemma \ref{lemma:alpha-mix-sum}, an identical argument shows we can pick $C_1$ large enough so that $\Pr\left(\mathcal{E}_2^c\right) \leq \frac{2}{\sqrt{\log^\delta T}}$ as well. Next, note that if $t < t_0$ and: 
\begin{align*}
    \left|\sum_{t'=t}^{t_0-1} z_{0,t'}\right| < \frac{C_1}{2}\sqrt{t_0-t}\log^{1+\frac{\delta}{4}} T
\end{align*}
and:
\begin{align*}
    \left|\sum_{t'=t_0}^{T} z_{1,t'}\right| < \frac{C_1}{2}\sqrt{T-t_0+1}\log^{1+\frac{\delta}{4}} T
\end{align*}
then:
\begin{align*}
    \left|\sum_{t'=t}^{T} z_{t'}\right| < \frac{C_1}{2}\sqrt{T-t+1}\log^{1+\frac{\delta}{4}} T + \frac{C_1}{2}\sqrt{t_0-t}\log^{1+\frac{\delta}{4}} T \leq C_1\sqrt{T-t+1}\log^{1+\frac{\delta}{4}} T. \tag{$T-t+1 > \max\{t_0-t,T-t_0+1\}$}
\end{align*}
So:
\small
\begin{align*}
     \Pr\left(\mathcal{E}^c_3\right) &\leq \Pr\left(\bigcup_{t=1}^{T} \left\{\left|\sum_{t'=t}^{T} z_{t'}\right| \geq C_1\sqrt{T-t+1}\log^{1+\frac{\delta}{4}} T\right\} \right) \\
     &\leq\Pr\left(\bigcup_{t=1}^{t_0-1} \left\{\left|\sum_{t'=t}^{T} z_{t'}\right| \geq C_1\sqrt{T-t+1}\log^{1+\frac{\delta}{4}} T\right\} \right) + \Pr\left(\bigcup_{t=t_0}^{T} \left\{\left|\sum_{t'=t}^{T} z_{1,t'}\right| \geq C_1\sqrt{T-t+1}\log^{1+\frac{\delta}{4}} T\right\} \right) \tag{union bound, $z_t = z_{1,t}$ for $t\geq t_0$} \\
     &\leq\Pr\left(\bigcup_{t=1}^{t_0-1} \left\{\left|\sum_{t'=t}^{t_0-1} z_{0,t'}\right| \geq \frac{C_1}{2}\sqrt{t_0-t}\log^{1+\frac{\delta}{4}} T\right\}\cup\left\{ \left|\sum_{t'=t_0}^{T} z_{1,t'}\right| \geq \frac{C_1}{2}\sqrt{T-t_0+1}\log^{1+\frac{\delta}{4}} T\right\}  \right) \\
     &\quad\: + \Pr\left(\bigcup_{t=t_0}^{T} \left\{\left|\sum_{t'=t}^{T} z_{1,t'}\right| \geq C_1\sqrt{T-t+1}\log^{1+\frac{\delta}{4}} T\right\} \right) \tag{union bound} \\
     &\leq \Pr\left(\bigcup_{t=1}^{t_0-1} \left\{\left|\sum_{t'=t}^{t_0-1} z_{0,t'}\right| \geq \frac{C_1}{2}\sqrt{t_0-t}\log^{1+\frac{\delta}{4}} T\right\}  \right) + \Pr\left( \left|\sum_{t'=t_0}^{T} z_{1,t'}\right| \geq \frac{C_1}{2}\sqrt{T-t_0+1}\log^{1+\frac{\delta}{4}} T  \right) \\
     &\quad\: + \Pr\left(\bigcup_{t=t_0}^{T} \left\{\left|\sum_{t'=t}^{T} z_{1,t'}\right| \geq C_1\sqrt{T-t+1}\log^{1+\frac{\delta}{4}} T\right\} \right) \tag{union bound} \\
\end{align*}
\normalsize
Once again, by Lemma \ref{lemma:alpha-mix-sum} there is some $K_3 > 0$ such that:
\begin{align*}
    \Pr\left(\bigcup_{t=1}^{T} \left\{\left|\sum_{t'=t}^{T} z_{1,t'}\right| \geq K_3\sqrt{T-t+1}\log^{1+\frac{\delta}{4}} T\right\} \right)  &\leq \frac{1}{\sqrt{\log^\delta T}}
\end{align*}
So for $C_1 \geq 2\max\{K_1,K_3\}$, we have $\Pr\left(\mathcal{E}_3^c\right) \leq \frac{3}{\sqrt{\log^\delta T}}$. Again, we can use an identical argument to show that we can pick $C_1$ large enough so that $\Pr\left(\mathcal{E}_4^c\right) \leq \frac{3}{\sqrt{\log^\delta T}}$.

\end{proof}
