% document set up
\documentclass{article}
\usepackage[utf8]{inputenc}
\usepackage{fullpage}
\setlength{\parindent}{0cm}
\setlength{\parskip}{1em}

% math packages
\usepackage{amsfonts}
\usepackage{amsmath}
\usepackage{amssymb}
\usepackage{amsthm}
\usepackage{enumitem}
\usepackage{bbm}

% general packages
\usepackage[colorlinks=true,linkcolor=blue,citecolor=blue]{hyperref}
\usepackage{natbib}

\newcommand\indep{\perp\!\!\!\perp}
\newcommand{\sforall}{\;\forall\;}
\newcommand{\E}{\mathbb{E}}
\newcommand{\Var}{\text{Var}}
\newcommand{\Cov}{\text{Cov}}
\newcommand{\argmin}[1]{\underset{#1}{\text{arg min}}}
\newcommand{\argmax}[1]{\underset{#1}{\text{arg max}}}

\begin{document}
\begin{align*}
    p(\mathbf{y} \;|\; \gamma = t; \tau_0,u_0,v_0) &= \int \mathbb{P}(\mathbf{y} \:|\:b,s,\gamma = t) \:\; d\mathbb{P}(b,s;\tau_0, u_0, v_0) \\
    &= \int\int p(y \;|\; b, s, \gamma =t) p(b|s;\tau_0)p(s;u_0,v_0)\;db\;ds\\
    &= \int_{0}^\infty\int_{-\infty}^\infty (2\pi)^{-T/2} s^{(T-t+1)/2} \exp\left[-\frac{\sum_{t'=1}^{t-1} y_{t'}^2 + \sum_{t'=t}^{T} s(y_{t'} - b)^2}{2}\right]  \\
    &\quad\quad\quad\quad\quad\quad\quad  \times (2\pi s\tau_0)^{1/2}\exp\left[-\frac{\tau_0 s b^2}{2}\right] \\
    &\quad\quad\quad\quad\quad\quad\quad  \times\frac{v_0^{u_0}}{\Gamma(u_0)}s^{u_0- 1}\exp(-v_0 s) \; db\; ds \\
    &\propto \exp\left[-\frac{1}{2}\sum_{t'=1}^{t-1} y_{t'}^2\right] \int_{0}^\infty\int_{-\infty}^\infty s^{1/2}\exp\left[-\frac{s}{2}\left((T-t+1)b^2 - 2b\sum_{t'=t}^{T}y_{t'}\right)\right] \\
    &\quad\quad\quad\quad\quad\quad\quad\quad\quad\quad\quad\quad\quad   \times s^{u_0 + \frac{T-t+1}{2} - 1}\exp\left[-s \left(v_0 + \frac{1}{2}\sum_{t=t'}^Ty_{t'}^2\right)\right] \; db\; ds \\
    &= \exp\left[-\frac{1}{2}\sum_{t'=1}^{t-1} y_{t'}^2\right] \int_{0}^\infty\int_{-\infty}^\infty s^{1/2}\exp\left[-\frac{s\overline{\tau}_t}{2}\left(b - \overline{b}_{t}\right)^2\right] s^{\overline{u}_t  - 1}\exp\left[-s \overline{v}_t\right] \; db\; ds \tag{$\overline{\tau}_t = \tau_0 + T - t+1, \; \overline{b}_t = \overline{\tau}_t^{-1}\sum_{t'=t}^T y_{t'}, \;\overline{u}_t = u_0 + \frac{T-t+1}{2}, \;\overline{v}_t = v_0 +\frac{1}{2} \sum_{t'=t}^T y_{t'}^2 - \frac{\overline{\tau}_t\overline{b}_t^2}{2}$} \\ 
    &\propto \exp\left[-\frac{1}{2}\sum_{t'=1}^{t-1} y_{t'}^2\right] \overline{\tau}_t^{-1/2} \frac{\Gamma(\overline{u}_t)}{\overline{v}_t^{\overline{u}_T}} \int_{0}^\infty\int_{-\infty}^\infty p(b|s;\overline{b}_t,\overline{\tau}_t)p(s;\overline{u}_t,\overline{v}_t)\;db\;ds \\
    &= \exp\left[-\frac{1}{2}\sum_{t'=1}^{t-1} y_{t'}^2\right] \overline{\tau}_t^{-1/2} \frac{\Gamma(\overline{u}_t)}{\overline{v}_t^{\overline{u}_T}}. 
\end{align*}
Taking the log we get:
\begin{align*}
    \log p(\mathbf{y} \;|\; \gamma = t; \tau_0,u_0,v_0) &= -\frac{1}{2}\sum_{t'=1}^{t-1} y_{t'}^2 - \frac{1}{2} \log \overline{\tau}_t + \log \Gamma(\overline{u}_t) - \overline{u}_t\log \overline{v}_t \\
    &= -\frac{1}{2}\log(\tau_0 + T - t + 1) - \frac{1}{2}\sum_{t'=1}^{t-1} y_{t'}^2 + \log \Gamma\left(u_0 + \frac{T - t +1}{2}\right)  \\
    &\quad\: - \left(u_0 + \frac{T - t +1}{2}\right)\log\left[v_0 +\frac{1}{2}\sum_{t'=t}^T y_{t'}^2 - \frac{1}{2(\tau + T- t +1)}\left(\sum_{t'=t}^T y_{t'}\right)^2 \right] \\
    &\quad\: + C
\end{align*}


\end{document}