    \begin{align}
        \tilde{v}_{kt} &:= v_k + \frac{1}{2}\sum_{t'=t}^{T+B_r}\overline{\lambda}_{-kt'}\delta_{t'}, \label{eq:mod-v_k} \\
        \tilde{\pi}_{kt} &:\propto \pi_{kt} \exp\left(-\frac{1}{2}\sum_{t'=1}^{t-1}\overline{\lambda}_{-kt'}\delta_{t'}\right).
        \label{eq:mod-pi_k}
    \end{align}

    \begin{align}
        \tilde{v}_{jt} &:= v_j + \frac{1}{2}\sum_{t'=t}^{T+B_r}\overline{\lambda}_{-jt'}\delta_{-jt'}, \label{eq:mod-v_j} \\
        \tilde{\pi}_{jt} &:\propto \pi_{jt} \exp\left(-\frac{1}{2}\sum_{t'=1}^{t-1}\overline{\lambda}_{-jt'}\delta_{-jt'}\right). \label{eq:mod-pi_j}
    \end{align}